\documentclass{article}
\topmargin -15mm
\textheight 24truecm   
\textwidth 16truecm    
\oddsidemargin 5mm
\evensidemargin 5mm   
\setlength\parskip{10pt}
\pagestyle{empty}          
\usepackage{boxedminipage}
\usepackage{amsfonts}
\usepackage{amsmath} 
\usepackage{amssymb}
\usepackage{amsthm}
\usepackage{t1enc}
\usepackage[utf8]{inputenc}
\usepackage{amssymb}
\usepackage{tikz}
\usepackage{commath}
\usepackage{listings}
\usepackage{verbatim}
\usepackage[margin=1in]{geometry}
\usepackage{caption}
\usepackage{subcaption}
\newcommand*\diff{\mathop{}\!\mathrm{d}}
\renewcommand{\thesubsection}{\thesection.\alph{subsection}}

\title{Assignment II - Generalized Linear Models}
\author{Filip Schjerven, Håkon Verås}
\date{\today}

\begin{document}

\maketitle
\begin{abstract}
In this project we have created a R-package called myglm and used it to discuss and analyze the salary-dataset. This involves implementing the print-, anova-, summary- and the myglm(...)-functions, similarly to the lm-package.
\end{abstract}
\newpage

\section{}

\subsection{}
Since we like to study how the mortality rate due to lung cancer varies with smoking status, we want to model external factors as an offset. The factor "age" differs from the other factors in the way people has a natural increase in mortality rate when they get older. We therefore want to model "age" as an offset, so that it gives a natural increase in mortality for older people and doesn't add bias to other covariates.

\subsection{}
We have that
\begin{equation*}
Y_{i} \sim \text{Po}(\mu_{i}),
\end{equation*}
so the Likelihood-function of $\mu_{i}$ is
\begin{equation*}
	L(y_{1},...,y_{n}|\mu_{i}) = \prod_{j=1}^{n} P(Y_{i} = y_{j}) = \prod_{j=1}^{n} \frac{e^{-\mu_{i}}\mu_{i}^{y_{j}}}{y_{j}!} = \frac{e^{-n\mu_{i}} \mu_{i}^{\sum_{j=1}^{n} y_{j}} }{\prod_{j=1}^{n} y_{j}!}.
\end{equation*}
Further, the log-likelihood function can also be derived:
\begin{equation*}
\text{log}(L) = -n\mu_{i} + \left(\sum_{j=1}^{n} y_{j}\right)\text{log} (\mu_{i}) - \sum_{j = 1}^{n} \text{log}(y_{j}!)
\end{equation*}
\begin{equation*}
= -n\mu_{i} + \left(\sum_{j=1}^{n} y_{j}\right)(\text{offset}_{i} + \nu_{i}) - \sum_{j = 1}^{n} \text{log}(y_{j}!)
\end{equation*}
\begin{equation*}
= -n\mu_{i} + \left(\sum_{j=1}^{n} y_{j}\right)(\text{offset}_{i} + \boldsymbol{x_{i} \beta}) - \sum_{j = 1}^{n} \text{log}(y_{j}!)
\end{equation*}
Resonnementet og påfølgende likninger er jeg litt usikre på.
\begin{equation*}
\nu_{i} = \boldsymbol{x_{i} \beta}
\end{equation*}
\begin{equation*}
\text{log}(\mu_{i}) = \text{offset}_{i} + \nu_{i}
\end{equation*}
\begin{equation*}
\text{log}(\mu_{i}) = \boldsymbol{x_{i} \beta}
\end{equation*}

\section{}
\subsection{}

\end{document}